muck about with experiments doing symbolic execution
in a section with assumed initial values for registers. This seems to
fail when the instruction includes calls to functions on values. At
least when doing Eval compute on them. Maybe that's the wrong thing to
do? More work is needed.

compcert-1.8/ia32/Peephole.v
@@ -337,31 +337,31 @@ Proof.
  destruct (v PC). destruct (v0 PC). elimtype False. apply H0. reflexivity.
   
 
+Admitted.
 
-
-  case_eq (regs_eq v v0).  
-  intros. (* need lemma -- regs_eq v v0 = true -> v = v0 to allow rewrite. *)
-  apply regs_eq__eq in H. rewrite H. reflexivity.
-  intro.
-  f_equal.
-  f_equal.
+ (*  case_eq (regs_eq v v0).   *)
+ (*  intros. (* need lemma -- regs_eq v v0 = true -> v = v0 to allow rewrite. *) *)
+ (*  apply regs_eq__eq in H. rewrite H. reflexivity. *)
+ (*  intro. *)
+ (*  f_equal. *)
+ (*  f_equal. *)
   
 
 
-  apply regs_eq__eq.
-  apply regs_not_eq__not_eq in H. inversion H. 
-  contradiction H0.
-  assert (regs_eq v v0 = true).
+ (*  apply regs_eq__eq. *)
+ (*  apply regs_not_eq__not_eq in H. inversion H.  *)
+ (*  contradiction H0. *)
+ (*  assert (regs_eq v v0 = true). *)
 
-  induction x.
-    case_eq (v PC).
-    intros. rewrite <- H1.
-  Eval compute in ((Pregmap.init Vundef) PC).
- destruct (v PC). destruct (v0 PC). reflexivity. 
+ (*  induction x. *)
+ (*    case_eq (v PC). *)
+ (*    intros. rewrite <- H1. *)
+ (*  Eval compute in ((Pregmap.init Vundef) PC). *)
+ (* destruct (v PC). destruct (v0 PC). reflexivity.  *)
   
   
   
-
+End Status_Dec.
 
 (* the initial register state for a program:
 
@@ -369,3 +369,62 @@ Proof.
         # PC <- (symbol_offset ge p.(prog_main) Int.zero)
         # RA <- Vzero
         # ESP <- (Vptr Mem.nullptr Int.zero) *)
+
+
+(* Here I'll try again to show equivalence by assuming a fully
+populated set of registers in a Section and see if it works. *)
+
+Section test.
+
+  (* the initial values for each register *)
+  Variables eax ebx ecx edx esi edi ebp esp : val.
+  Variables xmm0 xmm1 xmm2 xmm3 xmm4 xmm5 xmm6 xmm7 : val.
+  Definition init_regs := (Pregmap.init Vundef)
+    # EAX <- eax
+    # EBX <- ebx.
+
+Eval simpl in (init_regs EAX). (* = init_regs EAX : val *)
+Eval compute in (init_regs EAX). (* = eax : val *)
+Eval compute in (init_regs # ECX <- ecx). (* = fun y : preg => if match ... *)
+Eval compute in ((init_regs # ECX <- ecx) ECX). (* = ecx : val *)
+Eval simpl in (Val.add eax ebx). (* = Val.add eax ebx *)
+(* Eval simpl in (Val.add eax ebx). (* = FAILS TO TERMINATE, looking for real values?? *)*)
+
+(* the above sort of blows things for this approach I think... *)
+
+End test.
+
+  
+
+(*Inductive ireg: Type :=
+  | EAX: ireg  | EBX: ireg  | ECX: ireg  | EDX: ireg
+  | ESI: ireg  | EDI: ireg  | EBP: ireg  | ESP: ireg.
+
+(** Floating-point registers, i.e. SSE2 registers *)
+
+Inductive freg: Type :=
+  | XMM0: freg  | XMM1: freg  | XMM2: freg  | XMM3: freg
+  | XMM4: freg  | XMM5: freg  | XMM6: freg  | XMM7: freg.
+
+Lemma ireg_eq: forall (x y: ireg), {x=y} + {x<>y}.
+Proof. decide equality. Defined.
+
+Lemma freg_eq: forall (x y: freg), {x=y} + {x<>y}.
+Proof. decide equality. Defined.
+
+(** Bits of the flags register.  [SOF] is a pseudo-bit representing
+  the "xor" of the [OF] and [SF] bits. *)
+
+Inductive crbit: Type := 
+  | ZF | CF | PF | SOF.
+
+(** All registers modeled here. *)
+
+Inductive preg: Type :=
+  | PC: preg                            (**r program counter *)
+  | IR: ireg -> preg                    (**r integer register *)
+  | FR: freg -> preg                    (**r XMM register *)
+  | ST0: preg                           (**r top of FP stack *)
+  | CR: crbit -> preg                   (**r bit of the flags register *)
+  | RA: preg.                   (**r pseudo-reg representing return address *)
+*) 
